base/coq/Free/Class/ShareableArgs.v
@@ -5,10 +5,9 @@ Class ShareableArgs (Shape : Type) (Pos : Shape -> Type)
   {
     shareArgs : A -> Free Shape Pos A
   }.
-(*
-Instance ShareableArgsDummy (Shape : Type) (Pos : Shape -> Type)
-                            (A : Type)
- : ShareableArgs Shape Pos A | 5 := {
-    shareArgs := pure
- }.
-*)
+
+(* ShareableArgs instance for functions. 
+   Effects inside of functions are not shared. *)
+Instance ShareableArgsFunc (Shape : Type) (Pos : Shape -> Type) (A B : Type)
+ : ShareableArgs Shape Pos (A -> B) :=
+  { shareArgs := pure }.
