base/coq/Prelude/Pair.v
@@ -35,22 +35,7 @@ End SecPair.
 
 Arguments pair_  {Shape} {Pos} {A} {B}.
 
-(* ShareableArgs instance for Pair *)
-
-Instance ShareableArgsPair {Shape : Type} {Pos : Shape -> Type} (A B : Type)
-                        `{Injectable Share.Shape Share.Pos Shape Pos}
-                        `{ShareableArgs Shape Pos A}
-                        `{ShareableArgs Shape Pos B}
-  : ShareableArgs Shape Pos (Pair Shape Pos A B) := {
-     shareArgs p := match p with
-                    | pair_ fx fy => cbneed Shape Pos fx >>= fun sx =>
-                                     cbneed Shape Pos fy >>= fun sy =>
-                                     (pure (pair_ sx sy)) 
-                    end
-   }.
-
 (* Normalform instance for Pair *)
-
 Section SecNFPair.
 
   Variable Shape : Type.
@@ -75,3 +60,16 @@ Section SecNFPair.
    := { nf' := nf'Pair }.
 
 End SecNFPair.
+
+(* ShareableArgs instance for Pair *)
+Instance ShareableArgsPair {Shape : Type} {Pos : Shape -> Type} (A B : Type)
+                        `{Injectable Share.Shape Share.Pos Shape Pos}
+                        `{SAA : ShareableArgs Shape Pos A}
+                        `{SAB : ShareableArgs Shape Pos B}
+  : ShareableArgs Shape Pos (Pair Shape Pos A B) := {
+     shareArgs p := match p with
+                    | pair_ fx fy => cbneed Shape Pos (@shareArgs Shape Pos A SAA) fx >>= fun sx =>
+                                     cbneed Shape Pos (@shareArgs Shape Pos B SAB) fy >>= fun sy =>
+                                     (pure (pair_ sx sy)) 
+                    end
+   }.
